Factor out function definitions from svtv-generalize and svtv-to-fsm into separate -defs books

books/centaur/sv/svtv/svtv-to-fsm.lisp
@@ -26,7 +26,7 @@
 (in-package "SV")
 
 (include-book "../svex/override-transparency-and-ovmonotonicity")
-(include-book "svtv-generalize-defs")
+(include-book "svtv-to-fsm-defs")
 (include-book "override-envlist-defs")
 (include-book "fsm-override-transparency")
 (include-book "override-thm-common")
@@ -297,315 +297,6 @@ In particular this requires
   
 (local (xdoc::set-default-parents svtv-to-fsm))
 
-(define svar/4vec-p (x)
-  :short "Recognizer for an object that is either an @(see svar) or @(see 4vec)"
-  (or (svar-p x) (4vec-p x)))
-
-(define svar/4vec-kind ((x svar/4vec-p))
-  :parents (svar/4vec-p)
-  :short "Kind function for svar/4vec type"
-  :returns (kind (and (symbolp kind)
-                      (not (booleanp kind)))
-                 :rule-classes :type-prescription)
-  :guard-hints ((and stable-under-simplificationp
-                     '(:in-theory (enable svar/4vec-p svar-p 4vec-p))))
-  (if (consp x)
-      (if (integerp (car x))
-          :4vec
-        :svar)
-    (if (integerp x) :4vec (if (mbt (and x t)) :svar :4vec)))
-  ///
-  (defthm svar/4vec-kind-possibilities
-    (or (equal (svar/4vec-kind x) :4vec)
-        (equal (svar/4vec-kind x) :svar))
-    :rule-classes ((:forward-chaining :trigger-terms ((svar/4vec-kind x)))))
-  
-  (defthm svar/4vec-p-when-when-kind-is-4vec
-    (implies (equal (svar/4vec-kind x) :4vec)
-             (equal (svar/4vec-p x) (4vec-p x)))
-    :hints(("Goal" :in-theory (enable svar/4vec-p svar-p))))
-
-  (defthm svar/4vec-p-when-when-kind-is-svar
-    (implies (equal (svar/4vec-kind x) :svar)
-             (equal (svar/4vec-p x) (svar-p x)))
-    :hints(("Goal" :in-theory (enable svar/4vec-p 4vec-p))))
-
-  (defthm svar/4vec-kind-when-svar-p
-    (implies (svar-p x)
-             (Equal (svar/4vec-kind x) :svar))
-    :hints(("Goal" :in-theory (enable svar-p))))
-
-  (defthm svar/4vec-kind-when-4vec-p
-    (implies (4vec-p x)
-             (Equal (svar/4vec-kind x) :4vec))
-    :hints(("Goal" :in-theory (enable 4vec-p)))))
-
-(defmacro svar/4vec-case (x &rest args)
-  (fty::kind-casemacro-fn x args
-                          '(svar/4vec-case svar/4vec-kind (:4vec 4vec) (:svar svar))))
-
-(define svar/4vec-fix ((x svar/4vec-p))
-  :returns (new-x svar/4vec-p :hints(("Goal" :in-theory (enable svar/4vec-p))))
-  :parents (svar/4vec-p)
-  :short "Fixing function for svar/4vec type"
-  :hooks nil
-  (mbe :logic (if (eq (svar/4vec-kind x) :4vec)
-                  (4vec-fix x)
-                (svar-fix x))
-       :exec x)
-  ///
-
-  (defthm svar/4vec-fix-when-svar/4vec-p
-    (implies (svar/4vec-p x)
-             (equal (svar/4vec-fix x) x)))
-
-  (fty::deffixtype svar/4vec :pred svar/4vec-p :fix svar/4vec-fix :equiv svar/4vec-equiv :define t)
-
-  (defthm svar/4vec-fix-when-kind-is-4vec
-    (implies (equal (svar/4vec-kind x) :4vec)
-             (equal (svar/4vec-fix x) (4vec-fix x))))
-  
-  (defthm svar/4vec-fix-when-kind-is-svar
-    (implies (equal (svar/4vec-kind x) :svar)
-             (equal (svar/4vec-fix x) (svar-fix x))))
-
-  (fty::deffixequiv svar/4vec-kind))
-
-
-(defthm svex-p-when-svar/4vec-p
-  (implies (svar/4vec-p x)
-           (svex-p x))
-  :hints(("Goal" :in-theory (enable svar/4vec-p svar-p 4vec-p svex-p))))
-
-(defthm svar/4vec-p-when-svex-p
-  (implies (and (not (svex-case x :call))
-                (svex-p x))
-           (svar/4vec-p x))
-  :hints(("Goal" :in-theory (enable svar/4vec-p svar-p 4vec-p svex-p svex-kind))))
-
-(defthm svar/4vec-fix-of-svex-fix
-  (implies (not (svex-case x :call))
-           (equal (svar/4vec-fix (svex-fix x))
-                  (svar/4vec-fix x)))
-  :hints(("Goal" :in-theory (enable svar/4vec-fix svex-fix svex-kind
-                                    svar/4vec-kind)
-          :expand ((svex-fix x)))))
-
-(defthmd svar/4vec-fix-in-terms-of-svex-fix
-  (implies (not (svex-case x :call))
-           (equal (svar/4vec-fix x)
-                  (svex-fix x)))
-  :hints(("Goal" :in-theory (enable svar/4vec-fix svex-fix svex-kind
-                                    svar/4vec-kind)
-          :expand ((svex-fix x)))))
-
-(defthmd svar/4vec-kind-when-svex-kind
-  (implies (not (svex-case x :call))
-           (equal (svar/4vec-kind x)
-                  (if (equal (svex-kind x) :quote) :4vec :svar)))
-  :hints(("Goal" :in-theory (enable svex-kind svar/4vec-kind))))
-
-(define svar/4vec-eval ((x svar/4vec-p) (env svex-env-p))
-  :returns (val 4vec-p)
-  (svar/4vec-case x
-    :4vec (4vec-fix x)
-    :svar (svex-env-lookup x env))
-  ///
-  (defthmd svar/4vec-eval-in-terms-of-svex-eval
-    (implies (not (svex-case x :call))
-             (equal (svar/4vec-eval x env)
-                    (svex-eval x env)))
-    :hints (("goal" :expand ((svex-eval x env))
-             :in-theory (enable svex-var->name svex-quote->val
-                                svar/4vec-kind-when-svex-kind))))
-
-  (defthm svar/4vec-eval-of-quote
-    (implies (syntaxp (quotep x))
-             (equal (svar/4vec-eval x env)
-                    (svar/4vec-case x
-                      :4vec (4vec-fix x)
-                      :svar (svex-env-lookup x env))))))
-
-(fty::defmap svar/4vec-alist :key-type svar :val-type svar/4vec-p :true-listp t)
-
-(defthm svex-alist-p-when-svar/4vec-alist-p
-  (implies (svar/4vec-alist-p x)
-           (svex-alist-p x))
-  :hints(("Goal" :in-theory (enable svar/4vec-alist-p svex-alist-p))))
-
-
-(defthm svar/4vec-alist-p-when-svex-alist-p
-  (implies (and (svex-alist-noncall-p x)
-                (svex-alist-p x))
-           (svar/4vec-alist-p x))
-  :hints(("Goal" :in-theory (enable svex-alist-noncall-p
-                                    svex-alist-p
-                                    svar/4vec-alist-p))))
-
-(defthm svar/4vec-alist-fix-of-svex-alist-fix
-  (implies (svex-alist-noncall-p x)
-           (equal (svar/4vec-alist-fix (svex-alist-fix x))
-                  (svar/4vec-alist-fix x)))
-  :hints(("Goal" :in-theory (enable svar/4vec-alist-fix svex-alist-fix
-                                    svex-alist-noncall-p
-                                    svar/4vec-fix-in-terms-of-svex-fix))))
-
-(defthmd svar/4vec-alist-fix-in-terms-of-svex-alist-fix
-  (implies (svex-alist-noncall-p x)
-           (equal (svar/4vec-alist-fix x)
-                  (svex-alist-fix x)))
-  :hints(("Goal" :in-theory (enable svar/4vec-alist-fix svex-alist-fix
-                                    svex-alist-noncall-p
-                                    svar/4vec-fix-in-terms-of-svex-fix))))
-
-(define svar/4vec-alist-eval ((x svar/4vec-alist-p) (env svex-env-p))
-  :returns (val svex-env-p)
-  (b* (((when (atom x)) nil)
-       ((unless (mbt (and (consp (car x)) (svar-p (caar x)))))
-        (svar/4vec-alist-eval (cdr x) env)))
-    (cons (cons (caar x) (svar/4vec-eval (cdar x) env))
-          (svar/4vec-alist-eval (cdr x) env)))
-  ///
-  (defthmd svar/4vec-alist-eval-in-terms-of-svex-alist-eval
-    (implies (svex-alist-noncall-p x)
-             (equal (svar/4vec-alist-eval x env)
-                    (svex-alist-eval x env)))
-    :hints(("Goal" :in-theory (enable svex-alist-eval
-                                      svex-alist-noncall-p
-                                      svar/4vec-eval-in-terms-of-svex-eval))))
-
-  (defret svex-env-lookup-of-<fn>
-    (equal (svex-env-lookup v val)
-           (let ((look (hons-assoc-equal (svar-fix v) (svar/4vec-alist-fix x))))
-             (if look
-                 (svar/4vec-eval (cdr look) env)
-               (4vec-x))))
-    :hints(("Goal" :in-theory (enable svex-env-lookup-of-cons))))
-  
-  (local (in-theory (enable svar/4vec-alist-fix))))
-       
-
-(fty::deflist svar/4vec-alistlist :elt-type svar/4vec-alist :true-listp t)
-
-(defthm svex-alistlist-p-when-svar/4vec-alistlist-p
-  (implies (svar/4vec-alistlist-p x)
-           (svex-alistlist-p x))
-  :hints(("Goal" :in-theory (enable svar/4vec-alistlist-p svex-alistlist-p))))
-
-
-(defthm svar/4vec-alistlist-p-when-svex-alistlist-p
-  (implies (and (svex-alistlist-noncall-p x)
-                (svex-alistlist-p x))
-           (svar/4vec-alistlist-p x))
-  :hints(("Goal" :in-theory (enable svex-alistlist-noncall-p
-                                    svex-alistlist-p
-                                    svar/4vec-alistlist-p))))
-
-(defthm svar/4vec-alistlist-fix-of-svex-alistlist-fix
-  (implies (svex-alistlist-noncall-p x)
-           (equal (svar/4vec-alistlist-fix (svex-alistlist-fix x))
-                  (svar/4vec-alistlist-fix x)))
-  :hints(("Goal" :in-theory (enable svar/4vec-alistlist-fix svex-alistlist-fix
-                                    svex-alistlist-noncall-p
-                                    svar/4vec-alist-fix-in-terms-of-svex-alist-fix))))
-
-(defthmd svar/4vec-alistlist-fix-in-terms-of-svex-alistlist-fix
-  (implies (svex-alistlist-noncall-p x)
-           (equal (svar/4vec-alistlist-fix x)
-                  (svex-alistlist-fix x)))
-  :hints(("Goal" :in-theory (enable svar/4vec-alistlist-fix svex-alistlist-fix
-                                    svex-alistlist-noncall-p
-                                    svar/4vec-alist-fix-in-terms-of-svex-alist-fix))))
-
-(define svar/4vec-alistlist-eval ((x svar/4vec-alistlist-p) (env svex-env-p))
-  :returns (val svex-envlist-p)
-  (if (atom x)
-      nil
-    (cons (svar/4vec-alist-eval (car x) env)
-          (svar/4vec-alistlist-eval (cdr x) env)))
-  ///
-  (defthmd svar/4vec-alistlist-eval-in-terms-of-svex-alistlist-eval
-    (implies (svex-alistlist-noncall-p x)
-             (equal (svar/4vec-alistlist-eval x env)
-                    (svex-alistlist-eval x env)))
-    :hints(("Goal" :in-theory (enable svex-alistlist-eval
-                                      svex-alistlist-noncall-p
-                                      svar/4vec-alist-eval-in-terms-of-svex-alist-eval)))))
-  
-
-
-
-(defprod lhprobe
-  :short "Product type bundling an LHS (some list of FSM signal segments), a
-time step, and a Boolean indicating signedness, signifying the concatenated
-value of those segments at that time."
-  :long "<p>These are used for mapping FSM signals to SVTV variables. The
-signedness is relevant because of peculiarities of SVTV theorems.  In SVTV
-runs, only a lower segment of the bits of any given variable are relevant, but
-theorems about SVTV runs tend to specify the signedness of the variable.  E.g.,
-many input variables are assumed unsigned-byte-p of some size, and
-override-test variables are usually assumed to be -1 or 0.  Thus we need to map
-the relevant portions of the FSM variables sometimes to unsigned and sometimes
-to signed values.</p>"
-  ((lhs lhs-p)
-   (stage natp :rule-classes :type-prescription)
-   (signedp booleanp :rule-classes :type-prescription))
-  :layout :fulltree)
-
-
-(defthm lhatom-eval-zero-when-envs-agree
-  (implies (svex-envs-agree (lhatom-vars x) env1 env2)
-           (equal (lhatom-eval-zero x env1)
-                  (lhatom-eval-zero x env2)))
-  :hints(("Goal" :in-theory (enable lhatom-eval-zero
-                                    lhatom-vars)
-          :expand ((:free (v) (svex-envs-agree (list v) env1 env2))))))
-
-(define lhs-eval-ext ((x lhs-p) (env svex-env-p))
-  :returns (val 4vec-p)
-  (if (atom x)
-      0
-    (if (atom (cdr x))
-        (4vec-sign-ext (2vec (lhrange->w (car x)))
-                       (lhatom-eval-zero (lhrange->atom (car x)) env))
-      (4vec-concat (2vec (lhrange->w (car x)))
-                   (lhatom-eval-zero (lhrange->atom (car x)) env)
-                   (lhs-eval-ext (cdr x) env))))
-  ///
-  (defcong svex-envs-similar equal (lhs-eval-ext x env) 2
-    :hints(("Goal" :in-theory (enable lhatom-eval-zero)))))
-
-(defthm lhs-eval-zero-when-envs-agree
-  (implies (svex-envs-agree (lhs-vars x) env1 env2)
-           (equal (lhs-eval-zero x env1)
-                  (lhs-eval-zero x env2)))
-  :hints(("Goal" :in-theory (enable lhs-eval-zero
-                                    lhs-vars))))
-
-(defthm lhs-eval-ext-when-envs-agree
-  (implies (svex-envs-agree (lhs-vars x) env1 env2)
-           (equal (lhs-eval-ext x env1)
-                  (lhs-eval-ext x env2)))
-  :hints(("Goal" :in-theory (enable lhs-eval-ext
-                                    lhs-vars))))
-
-(define svex-envlists-agree ((vars svarlist-p)
-                             (x svex-envlist-p)
-                             (y svex-envlist-p))
-  (if (atom x)
-      (atom y)
-    (and (consp y)
-         (svex-envs-agree vars (car x) (car y))
-         (svex-envlists-agree vars (cdr x) (cdr y))))
-  ///
-  (defthm svex-envs-agree-nth-when-svex-envlists-agree
-    (implies (svex-envlists-agree vars x y)
-             (svex-envs-agree vars (nth n x) (nth n y))))
-
-  (defthm svex-envlists-agree-of-append-vars
-    (iff (svex-envlists-agree (append vars1 vars2) x y)
-         (and (svex-envlists-agree vars1 x y)
-              (svex-envlists-agree vars2 x y)))))
 
 
 ;; (define lhprobe-eval-ext ((x lhprobe-p)
@@ -621,290 +312,6 @@ to signed values.</p>"
          (equal (nth n (svex-envlist-fix x))
                 (svex-env-fix (nth n x)))
          :hints(("Goal" :in-theory (enable svex-envlist-fix)))))
-
-(define lhprobe-eval ((x lhprobe-p)
-                      (envs svex-envlist-p))
-  :parents (lhprobe)
-  :short "Evaluator for an @(see lhprobe) with respect to an envlist giving the values of signals over time."
-  :returns (val 4vec-p)
-  (b* (((lhprobe x))
-       (env (nth x.stage envs)))
-    (if x.signedp
-        (lhs-eval-ext x.lhs env)
-      (lhs-eval-zero x.lhs env)))
-  ///
-  (defthm lhprobe-eval-of-take
-    (implies (< (lhprobe->stage x) (nfix n))
-             (equal (lhprobe-eval x (take n envs))
-                    (lhprobe-eval x envs)))))
-
-
-
-(define lhprobe-vars ((x lhprobe-p))
-  :parents (lhprobe)
-  :short "Collect variables present in an lhprobe"
-  :returns (vars svarlist-p)
-  (b* (((lhprobe x)))
-    (lhs-vars x.lhs))
-  ///
-
-
-  (defthm svex-env-extract-nil-under-svex-envs-similar
-    (svex-envs-similar (svex-env-extract vars nil) nil)
-    :hints(("Goal" :in-theory (enable svex-envs-similar))))
-  
-  (defthm nth-of-svex-envlist-extract
-    (svex-envs-similar (nth n (svex-envlist-extract-keys vars x))
-                       (svex-env-extract vars (nth n x)))
-    :hints(("Goal" :in-theory (enable svex-envlist-extract-keys))))
-
-
-  (defthm lhs-eval-ext-of-svex-env-extract
-    (implies (subsetp-equal (lhs-vars x) (Svarlist-fix vars))
-             (equal (lhs-eval-ext x (svex-env-extract vars env))
-                    (lhs-eval-ext x env)))
-    :hints(("Goal" :in-theory (enable lhs-eval-ext
-                                      lhatom-vars
-                                      lhatom-eval-zero))))
-
-  (defthm lhs-eval-zero-of-svex-env-extract
-    (implies (subsetp-equal (lhs-vars x) (Svarlist-fix vars))
-             (equal (lhs-eval-zero x (svex-env-extract vars env))
-                    (lhs-eval-zero x env)))
-    :hints(("Goal" :in-theory (enable lhs-eval-zero
-                                      lhatom-vars
-                                      lhatom-eval-zero))))
-  
-  (defthm lhprobe-eval-of-svex-envlist-extract-vars
-    (implies (subsetp-equal (lhprobe-vars x) (Svarlist-fix vars))
-             (equal (lhprobe-eval x (svex-envlist-extract-keys vars envs))
-                    (lhprobe-eval x envs)))
-    :hints(("Goal" :in-theory (enable lhprobe-eval))))
-
-  (defthm lhprobe-eval-when-envs-agree
-    (implies (svex-envlists-agree (lhprobe-vars x) envs1 envs2)
-             (equal (lhprobe-eval x envs1)
-                    (lhprobe-eval x envs2)))
-    :hints(("Goal" :in-theory (enable lhprobe-eval
-                                      lhprobe-vars))
-           (and stable-under-simplificationp
-                '(:use ((:instance lhs-eval-ext-when-envs-agree
-                         (x (lhprobe->lhs x))
-                         (env1 (nth (lhprobe->stage x) envs1))
-                         (env2 (nth (lhprobe->stage x) envs2)))
-                        (:instance lhs-eval-zero-when-envs-agree
-                         (x (lhprobe->lhs x))
-                         (env1 (nth (lhprobe->stage x) envs1))
-                         (env2 (nth (lhprobe->stage x) envs2)))))))))
-
-
-(define lhprobe-change-override ((x lhprobe-p)
-                                 (type svar-overridetype-p))
-  :returns (new-x lhprobe-p)
-  (change-lhprobe x :lhs (lhs-change-override (lhprobe->lhs x) type)))
-
-
-
-(fty::defmap lhprobe-map :key-type svar :val-type lhprobe :true-listp t
-  :short "Mapping from variables to lhprobes, identifying SVTV variables with signals at a time")
-
-(define lhprobe-map-eval ((x lhprobe-map-p)
-                          (envs svex-envlist-p))
-  :returns (eval svex-env-p)
-  (b* (((when (atom x))
-        nil)
-       ((unless (mbt (and (consp (car x)) (svar-p (caar x)))))
-        (lhprobe-map-eval (cdr x) envs)))
-    (cons (cons (caar x) (lhprobe-eval (cdar x) envs))
-          (lhprobe-map-eval (cdr x) envs)))
-  ///
-  (defret lookup-of-<fn>
-    (equal (svex-env-lookup v eval)
-           (let ((look (hons-assoc-equal (svar-fix v) (lhprobe-map-fix x))))
-             (if look
-                 (lhprobe-eval (cdr look) envs)
-               (4vec-x))))
-    :hints(("Goal" :in-theory (enable svex-env-lookup-of-cons))))
-  (local (in-theory (enable lhprobe-map-fix))))
-
-
-(define lhprobe-map-vars ((x lhprobe-map-p))
-  :parents (lhprobe)
-  :short "Collect variables present in an lhprobe-map"
-  :returns (vars svarlist-p)
-  (b* (((when (atom x))
-        nil)
-       ((unless (mbt (and (consp (car x)) (svar-p (caar x)))))
-        (lhprobe-map-vars (cdr x))))
-    (append (lhprobe-vars (cdar x))
-            (lhprobe-map-vars (cdr x))))
-  ///
-
-  (defthm lhprobe-map-eval-of-svex-envlist-extract-vars
-    (implies (subsetp-equal (lhprobe-map-vars x) (Svarlist-fix vars))
-             (equal (lhprobe-map-eval x (svex-envlist-extract-keys vars envs))
-                    (lhprobe-map-eval x envs)))
-    :hints(("Goal" :in-theory (enable lhprobe-map-eval))))
-
-  (local (in-theory (enable lhprobe-map-fix)))
-
-  (defthm lhprobe-map-eval-when-envs-agree
-    (implies (svex-envlists-agree (lhprobe-map-vars x) envs1 envs2)
-             (equal (lhprobe-map-eval x envs1)
-                    (lhprobe-map-eval x envs2)))
-    :hints(("Goal" :in-theory (enable lhprobe-map-eval
-                                      lhprobe-map-vars)))))
-       
-
-
-(define lhprobe/4vec-p (x)
-  :short "Recognizer for an object that is either a @(see lhprobe) or @(see 4vec)."
-  (or (lhprobe-p x) (4vec-p x)))
-
-(define lhprobe/4vec-kind ((x lhprobe/4vec-p))
-  :parents (lhprobe/4vec-p)
-  :short "Kind function for lhprobe/4vec type"
-  :returns (kind (and (symbolp kind)
-                      (not (booleanp kind)))
-                 :rule-classes :type-prescription)
-  (if (or (atom x)
-          (integerp (car x)))
-      :4vec
-    :lhprobe)
-  ///
-  (defthm lhprobe/4vec-kind-possibilities
-    (or (equal (lhprobe/4vec-kind x) :4vec)
-        (equal (lhprobe/4vec-kind x) :lhprobe))
-    :rule-classes ((:forward-chaining :trigger-terms ((lhprobe/4vec-kind x)))))
-  
-  (defthm lhprobe/4vec-p-when-when-kind-is-4vec
-    (implies (equal (lhprobe/4vec-kind x) :4vec)
-             (equal (lhprobe/4vec-p x) (4vec-p x)))
-    :hints(("Goal" :in-theory (enable lhprobe/4vec-p lhprobe-p))))
-
-  (defthm lhprobe/4vec-p-when-when-kind-is-lhprobe
-    (implies (equal (lhprobe/4vec-kind x) :lhprobe)
-             (equal (lhprobe/4vec-p x) (lhprobe-p x)))
-    :hints(("Goal" :in-theory (enable lhprobe/4vec-p 4vec-p))))
-
-  (defthm lhprobe/4vec-kind-when-lhprobe-p
-    (implies (lhprobe-p x)
-             (Equal (lhprobe/4vec-kind x) :lhprobe))
-    :hints(("Goal" :in-theory (enable lhprobe-p))))
-
-  (defthm lhprobe/4vec-kind-when-4vec-p
-    (implies (4vec-p x)
-             (Equal (lhprobe/4vec-kind x) :4vec))
-    :hints(("Goal" :in-theory (enable 4vec-p)))))
-
-(defmacro lhprobe/4vec-case (x &rest args)
-  (fty::kind-casemacro-fn x args
-                          '(lhprobe/4vec-case lhprobe/4vec-kind (:4vec 4vec) (:lhprobe lhprobe))))
-
-(define lhprobe/4vec-fix ((x lhprobe/4vec-p))
-  :parents (lhprobe/4vec-p)
-  :hooks nil
-  :short "Fixing function for lhprobe/4vec type"
-  :returns (new-x lhprobe/4vec-p :hints(("Goal" :in-theory (enable lhprobe/4vec-p))))
-  (mbe :logic (if (eq (lhprobe/4vec-kind x) :4vec)
-                  (4vec-fix x)
-                (lhprobe-fix x))
-       :exec x)
-  ///
-
-  (defthm lhprobe/4vec-fix-when-lhprobe/4vec-p
-    (implies (lhprobe/4vec-p x)
-             (equal (lhprobe/4vec-fix x) x)))
-
-  (fty::deffixtype lhprobe/4vec :pred lhprobe/4vec-p :fix lhprobe/4vec-fix :equiv lhprobe/4vec-equiv :define t)
-
-  (defthm lhprobe/4vec-fix-when-kind-is-4vec
-    (implies (equal (lhprobe/4vec-kind x) :4vec)
-             (equal (lhprobe/4vec-fix x) (4vec-fix x))))
-  
-  (defthm lhprobe/4vec-fix-when-kind-is-lhprobe
-    (implies (equal (lhprobe/4vec-kind x) :lhprobe)
-             (equal (lhprobe/4vec-fix x) (lhprobe-fix x))))
-
-  (fty::deffixequiv lhprobe/4vec-kind))
-
-(define lhprobe/4vec-eval ((x lhprobe/4vec-p)
-                           (envs svex-envlist-p))
-  :short "Evaluator for @(see lhprobe/4vec-p) objects"
-  :parents (lhprobe/4vec-p)
-  :returns (val 4vec-p)
-  (lhprobe/4vec-case x
-    :lhprobe (lhprobe-eval x envs)
-    :4vec (4vec-fix x)))
-
-
-(define lhprobe/4vec-vars ((x lhprobe/4vec-p))
-  :parents (lhprobe)
-  :short "Collect variables present in an lhprobe/4vec"
-  :returns (vars svarlist-p)
-  (lhprobe/4vec-case x
-    :4vec nil
-    :lhprobe (lhprobe-vars x))
-  ///
-
-
-  
-  (defthm lhprobe/4vec-eval-of-svex-envlist-extract-vars
-    (implies (subsetp-equal (lhprobe/4vec-vars x) (Svarlist-fix vars))
-             (equal (lhprobe/4vec-eval x (svex-envlist-extract-keys vars envs))
-                    (lhprobe/4vec-eval x envs)))
-    :hints(("Goal" :in-theory (enable lhprobe/4vec-eval)))))
-
-(define lhprobe/4vec-change-override ((x lhprobe/4vec-p)
-                                      (type svar-overridetype-p))
-  :returns (new-x lhprobe/4vec-p)
-  (lhprobe/4vec-case x
-    :4vec (4vec-fix x)
-    :lhprobe (lhprobe-change-override x type)))
-
-
-
-
-
-(defprod lhprobe-constraint
-  :short "Constraint equating an @(see lhprobe) (that is, a concatenation of signals at some time) equals either a @(see 4vec) constant or the value of another lhprobe."
-  ((lhprobe lhprobe-p)
-   (val lhprobe/4vec-p))
-  :layout :fulltree)
-
-(fty::deflist lhprobe-constraintlist :elt-type lhprobe-constraint-p :true-listp t)
-
-
-(define lhprobe-constraint-eval ((x lhprobe-constraint-p)
-                                 (envs svex-envlist-p))
-  (b* (((lhprobe-constraint x)))
-    (equal (lhprobe-eval x.lhprobe envs)
-           (lhprobe/4vec-eval x.val envs))))
-
-(define lhprobe-constraintlist-eval ((x lhprobe-constraintlist-p)
-                                     (envs svex-envlist-p))
-  (if (atom x)
-      t
-    (and (lhprobe-constraint-eval (car x) envs)
-         (lhprobe-constraintlist-eval (cdr x) envs)))
-  ///
-  (defthm lhprobe-constraintlist-eval-of-append
-    (equal (lhprobe-constraintlist-eval (append x y) envs)
-           (and (lhprobe-constraintlist-eval x envs)
-                (lhprobe-constraintlist-eval y envs)))))
-
-(define lhatom-overridemux-eval ((x lhatom-p)
-                                 (env svex-env-p)
-                                 (out svex-env-p))
-  :returns (val 4vec-p)
-  (lhatom-case x
-    :z 0
-    :var (4vec-rsh (2vec x.rsh)
-                   (if (svar-override-p x.name :val)
-                       (4vec-bit?! (svex-env-fastlookup (svar-change-override x.name :test) env)
-                                   (svex-env-fastlookup x.name env)
-                                   (svex-env-fastlookup (svar-change-override x.name nil) out))
-                     (svex-env-fastlookup x.name env)))))
 
 
 (local (defthm 4vec-bit?!-of-4vec-concat
@@ -932,21 +339,10 @@ to signed values.</p>"
          :hints (("goal" :in-theory (enable 4vec-sign-ext 4vec-shift-core 4vec-bit?! 4vec-bitmux 4vec-1mask))
                  (bitops::logbitp-reasoning))))
 
-(define lhs-overridemux-eval-ext ((x lhs-p)
-                              (env svex-env-p)
-                              (out svex-env-p))
-  :returns (val 4vec-p)
-  (if (atom x)
-      0
-    (if (atom (cdr x))
-        (4vec-sign-ext (2vec (lhrange->w (car x)))
-                       (lhatom-overridemux-eval (lhrange->atom (car x)) env out))
-      (4vec-concat (2vec (lhrange->w (car x)))
-                   (lhatom-overridemux-eval (lhrange->atom (car x)) env out)
-                   (lhs-overridemux-eval-ext (cdr x) env out))))
-  ///
 
 
+(defsection lhs-overridemux-eval-ext
+  (local (in-theory (enable lhs-overridemux-eval-ext)))
   (defthm lhs-overridemux-eval-ext-when-overridetype
     (implies (svarlist-override-p (lhs-vars x) type)
              (equal (lhs-overridemux-eval-ext x env out)
@@ -986,16 +382,6 @@ to signed values.</p>"
                                     (lhs-eval-ext (lhs-change-override x nil) out))
                       (lhs-eval-ext x env)))))
 
-  (defthm lhs-vars-of-lhs-change-override
-    (equal (lhs-vars (lhs-change-override x type))
-           (svarlist-change-override (lhs-vars x) type))
-    :hints(("Goal" :in-theory (enable svarlist-change-override lhs-change-override lhatom-change-override lhs-vars lhatom-vars))))
-
-  (defthm lhs-change-override-of-lhs-change-override
-    (equal (lhs-change-override (lhs-change-override x type1) type2)
-           (lhs-change-override x type2))
-    :hints(("Goal" :in-theory (enable lhs-change-override lhatom-change-override))))
-  
   (defthm lhs-overridemux-eval-ext-of-lhs-change-override
     (equal (lhs-overridemux-eval-ext (lhs-change-override x type) env out)
            (if (svar-overridetype-equiv type :val)
@@ -1007,17 +393,8 @@ to signed values.</p>"
                            (vars (lhs-vars (lhs-change-override x type)))
                            (x (lhs-change-override x type))))))))
 
-(define lhs-overridemux-eval-zero ((x lhs-p)
-                              (env svex-env-p)
-                              (out svex-env-p))
-  :returns (val 4vec-p)
-  (if (atom x)
-      0
-    (4vec-concat (2vec (lhrange->w (car x)))
-                 (lhatom-overridemux-eval (lhrange->atom (car x)) env out)
-                 (lhs-overridemux-eval-zero (cdr x) env out)))
-  ///
-
+(defsection lhs-overridemux-eval-zero
+  (local (in-theory (enable lhs-overridemux-eval-zero)))
 
   (defthm lhs-overridemux-eval-zero-when-overridetype
     (implies (svarlist-override-p (lhs-vars x) type)
@@ -1057,16 +434,6 @@ to signed values.</p>"
                                     (lhs-eval-zero x env)
                                     (lhs-eval-zero (lhs-change-override x nil) out))
                       (lhs-eval-zero x env)))))
-
-  (defthm lhs-vars-of-lhs-change-override
-    (equal (lhs-vars (lhs-change-override x type))
-           (svarlist-change-override (lhs-vars x) type))
-    :hints(("Goal" :in-theory (enable svarlist-change-override lhs-change-override lhatom-change-override lhs-vars lhatom-vars))))
-
-  (defthm lhs-change-override-of-lhs-change-override
-    (equal (lhs-change-override (lhs-change-override x type1) type2)
-           (lhs-change-override x type2))
-    :hints(("Goal" :in-theory (enable lhs-change-override lhatom-change-override))))
   
   (defthm lhs-overridemux-eval-zero-of-lhs-change-override
     (equal (lhs-overridemux-eval-zero (lhs-change-override x type) env out)
@@ -1079,19 +446,8 @@ to signed values.</p>"
                            (vars (lhs-vars (lhs-change-override x type)))
                            (x (lhs-change-override x type))))))))
 
-
-(define lhprobe-overridemux-eval ((x lhprobe-p)
-                                  (envs svex-envlist-p)
-                                  (outs svex-envlist-p))
-  :returns (val 4vec-p)
-  (b* (((lhprobe x))
-       (env (nth x.stage envs))
-       (out (nth x.stage outs)))
-    (if x.signedp
-        (lhs-overridemux-eval-ext x.lhs env out)
-      (lhs-overridemux-eval-zero x.lhs env out)))
-  ///
-
+(defsection lhprobe-overridemux-eval
+  (local (in-theory (enable lhprobe-overridemux-eval)))
   (defthm lhprobe-overridemux-eval-when-overridetype
     (implies (svarlist-override-p (lhprobe-vars x) type)
              (equal (lhprobe-overridemux-eval x env out)
@@ -1138,14 +494,8 @@ to signed values.</p>"
     :hints(("Goal" :in-theory (disable lhprobe-overridemux-eval)))))
 
 
-(define lhprobe/4vec-overridemux-eval ((x lhprobe/4vec-p)
-                                       (envs svex-envlist-p)
-                                       (outs svex-envlist-p))
-  :returns (val 4vec-p)
-  (lhprobe/4vec-case x
-    :lhprobe (lhprobe-overridemux-eval x envs outs)
-    :4vec (4vec-fix x))
-  ///
+(defsection lhprobe/4vec-overridemux-eval
+  (local (in-theory (enable lhprobe/4vec-overridemux-eval)))
   (local (defthm 4vec-bit?!-self
            (equal (4vec-bit?! y x x)
                   (4vec-fix x))
@@ -1188,53 +538,8 @@ to signed values.</p>"
                       (lhprobe/4vec-eval x env))))
     :hints(("Goal" :in-theory (disable lhprobe/4vec-overridemux-eval)))))
 
-(define lhprobe-constraint-overridemux-eval ((x lhprobe-constraint-p)
-                                             (envs svex-envlist-p)
-                                             (outs svex-envlist-p))
-  (b* (((lhprobe-constraint x)))
-    (equal (lhprobe-overridemux-eval x.lhprobe envs outs)
-           (lhprobe/4vec-overridemux-eval x.val envs outs))))
-
-(define lhprobe-constraintlist-overridemux-eval ((x lhprobe-constraintlist-p)
-                                                 (envs svex-envlist-p)
-                                                 (outs svex-envlist-p))
-  (if (atom x)
-      t
-    (and (lhprobe-constraint-overridemux-eval (car x) envs outs)
-         (lhprobe-constraintlist-overridemux-eval (cdr x) envs outs)))
-  ///
-  (defthm lhprobe-constraintlist-overridemux-eval-of-append
-    (equal (lhprobe-constraintlist-overridemux-eval (append x y) envs outs)
-           (and (lhprobe-constraintlist-overridemux-eval x envs outs)
-                (lhprobe-constraintlist-overridemux-eval y envs outs)))))
-
-
-(define lhprobe-map-overridemux-eval ((x lhprobe-map-p)
-                                      (envs svex-envlist-p)
-                                      (outs svex-envlist-p))
-  :returns (eval svex-env-p)
-  (b* (((when (atom x))
-        nil)
-       ((unless (mbt (and (consp (car x)) (svar-p (caar x)))))
-        (lhprobe-map-overridemux-eval (cdr x) envs outs)))
-    (cons (cons (caar x) (lhprobe-overridemux-eval (cdar x) envs outs))
-          (lhprobe-map-overridemux-eval (cdr x) envs outs)))
-  ///
-  (defret lookup-of-<fn>
-    (equal (svex-env-lookup v eval)
-           (let ((look (hons-assoc-equal (svar-fix v) (lhprobe-map-fix x))))
-             (if look
-                 (lhprobe-overridemux-eval (cdr look) envs outs)
-               (4vec-x))))
-    :hints(("Goal" :in-theory (enable svex-env-lookup-of-cons))))
-
-  (defret boundp-of-<fn>
-    (iff (svex-env-boundp v eval)
-         (hons-assoc-equal (svar-fix v) (lhprobe-map-fix x)))
-    :hints(("Goal" :in-theory (enable svex-env-boundp-of-cons-split))))
-  
-  (local (in-theory (enable lhprobe-map-fix)))
-
+(defsection lhprobe-map-overridemux-eval
+  (local (in-theory (enable lhprobe-map-overridemux-eval)))
   (defthm lhprobe-map-overridemux-eval-when-overridetype
     (implies (and (svarlist-override-p (lhprobe-map-vars x) type)
                   (not (equal (svar-overridetype-fix type) :val)))
@@ -1246,236 +551,6 @@ to signed values.</p>"
 
 
 
-(define lhprobe-map-max-stage ((x lhprobe-map-p))
-  :returns (stage integerp :rule-classes :type-prescription)
-  (if (atom x)
-      -1
-    (if (mbt (and (consp (car x)) (svar-p (caar x))))
-        (max (lhprobe->stage (cdar x))
-             (lhprobe-map-max-stage (cdr x)))
-      (lhprobe-map-max-stage (cdr x))))
-  ///
-  (local (in-theory (disable nth take acl2::take-of-len-free acl2::take-when-atom acl2::take-of-too-many)))
-
-  (defthm lhprobe-map-overridemux-eval-of-take-envs
-    (implies (< (lhprobe-map-max-stage x) (nfix n))
-             (equal (lhprobe-map-overridemux-eval x (take n envs) outs)
-                    (lhprobe-map-overridemux-eval x envs outs)))
-    :hints(("Goal" :in-theory (enable lhprobe-map-overridemux-eval
-                                      lhprobe-overridemux-eval
-                                      lhprobe/4vec-overridemux-eval))))
-  (defthm lhprobe-map-overridemux-eval-of-take-outs
-    (implies (< (lhprobe-map-max-stage x) (nfix n))
-             (equal (lhprobe-map-overridemux-eval x envs (take n outs))
-                    (lhprobe-map-overridemux-eval x envs outs)))
-    :hints(("Goal" :in-theory (enable lhprobe-map-overridemux-eval
-                                      lhprobe-overridemux-eval
-                                      lhprobe/4vec-overridemux-eval))))
-
-  (defthm lhprobe-map-eval-of-take-outs
-    (implies (< (lhprobe-map-max-stage x) (nfix n))
-             (equal (lhprobe-map-eval x (take n envs))
-                    (lhprobe-map-eval x envs)))
-    :hints(("Goal" :in-theory (enable lhprobe-map-eval
-                                      lhprobe-eval
-                                      lhprobe/4vec-eval))))
-
-  (defthm lhprobe->stage-of-lookup-bound
-    (implies (hons-assoc-equal v (lhprobe-map-fix x))
-             (<= (lhprobe->stage (cdr (hons-assoc-equal v x)))
-                 (lhprobe-map-max-stage x)))
-    :rule-classes :linear)
-
-  (defthm lhprobe-map-max-stage-lower-bound
-    (<= -1 (lhprobe-map-max-stage x))
-    :rule-classes :linear)
-  
-  (local (in-theory (enable lhprobe-map-fix))))
-
-(define lhprobe-constraint-max-stage ((x lhprobe-constraint-p))
-  :returns (stage natp :rule-classes :type-prescription)
-  (b* (((lhprobe-constraint x)))
-    (if (lhprobe/4vec-case x.val :lhprobe)
-        (max (lhprobe->stage (lhprobe/4vec-fix x.val)) (lhprobe->stage x.lhprobe))
-      (lhprobe->stage x.lhprobe)))
-  ///
-  (local (in-theory (disable nth take acl2::take-of-len-free acl2::take-when-atom acl2::take-of-too-many)))
-
-  (defthm lhprobe-constraint-overridemux-eval-of-take-envs
-    (implies (< (lhprobe-constraint-max-stage x) (nfix n))
-             (equal (lhprobe-constraint-overridemux-eval x (take n envs) outs)
-                    (lhprobe-constraint-overridemux-eval x envs outs)))
-    :hints(("Goal" :in-theory (enable lhprobe-constraint-overridemux-eval
-                                      lhprobe-overridemux-eval
-                                      lhprobe/4vec-overridemux-eval))))
-  (defthm lhprobe-constraint-overridemux-eval-of-take-outs
-    (implies (< (lhprobe-constraint-max-stage x) (nfix n))
-             (equal (lhprobe-constraint-overridemux-eval x envs (take n outs))
-                    (lhprobe-constraint-overridemux-eval x envs outs)))
-    :hints(("Goal" :in-theory (enable lhprobe-constraint-overridemux-eval
-                                      lhprobe-overridemux-eval
-                                      lhprobe/4vec-overridemux-eval))))
-
-  (defthm lhprobe-constraint-eval-of-take-outs
-    (implies (< (lhprobe-constraint-max-stage x) (nfix n))
-             (equal (lhprobe-constraint-eval x (take n envs))
-                    (lhprobe-constraint-eval x envs)))
-    :hints(("Goal" :in-theory (enable lhprobe-constraint-eval
-                                      lhprobe-eval
-                                      lhprobe/4vec-eval)))))
-
-
-(define lhprobe-constraintlist-max-stage ((x lhprobe-constraintlist-p))
-  :returns (stage integerp :rule-classes :type-prescription)
-  (if (atom x)
-      -1
-    (max (lhprobe-constraint-max-stage (car x))
-         (lhprobe-constraintlist-max-stage (cdr x))))
-  ///
-  (local (in-theory (disable nth take acl2::take-of-len-free acl2::take-when-atom acl2::take-of-too-many)))
-  
-  (defthm lhprobe-constraintlist-overridemux-eval-of-take-envs
-    (implies (< (lhprobe-constraintlist-max-stage x) (nfix n))
-             (equal (lhprobe-constraintlist-overridemux-eval x (take n envs) outs)
-                    (lhprobe-constraintlist-overridemux-eval x envs outs)))
-    :hints(("Goal" :in-theory (enable lhprobe-constraintlist-overridemux-eval))))
-  
-  (defthm lhprobe-constraintlist-overridemux-eval-of-take-outs
-    (implies (< (lhprobe-constraintlist-max-stage x) (nfix n))
-             (equal (lhprobe-constraintlist-overridemux-eval x envs (take n outs))
-                    (lhprobe-constraintlist-overridemux-eval x envs outs)))
-    :hints(("Goal" :in-theory (enable lhprobe-constraintlist-overridemux-eval))))
-
-  (defthm lhprobe-constraintlist-eval-of-take-outs
-    (implies (< (lhprobe-constraintlist-max-stage x) (nfix n))
-             (equal (lhprobe-constraintlist-eval x (take n envs))
-                    (lhprobe-constraintlist-eval x envs)))
-    :hints(("Goal" :in-theory (enable lhprobe-constraintlist-eval))))
-
-  (defthm lhprobe-constraintlist-max-stage-lower-bound
-    (<= -1 (lhprobe-constraintlist-max-stage x))
-    :rule-classes :linear)
-  
-  (defthm lhprobe-constraintlist-max-stage-of-append
-    (Equal (lhprobe-constraintlist-max-stage (append x y))
-           (max (lhprobe-constraintlist-max-stage x)
-                (lhprobe-constraintlist-max-stage y)))))
-
-
-
-(define svtv-spec-fsm-bindings-for-lhprobe ((lhprobe lhprobe-p)
-                                            (binding svar/4vec-p)
-                                            (bindings-acc lhprobe-map-p))
-  :returns (bindings lhprobe-map-p)
-  (svar/4vec-case binding
-    :4vec (lhprobe-map-fix bindings-acc)
-    :svar
-    ;; svtv variable, add a binding unless there is one already
-    (b* ((binding-look (hons-get (svar-fix binding) (lhprobe-map-fix bindings-acc)))
-         ((unless binding-look)
-          (hons-acons (svar-fix binding) (lhprobe-fix lhprobe)
-                      (lhprobe-map-fix bindings-acc))))
-      (lhprobe-map-fix bindings-acc)))
-  ///
-  (defret lhprobe-map-max-stage-of-<fn>
-    (implies (and (<= (lhprobe->stage lhprobe) bound)
-                  (<= (lhprobe-map-max-stage bindings-acc) bound))
-             (<= (lhprobe-map-max-stage bindings) bound))
-    :hints(("Goal" :in-theory (enable lhprobe-map-max-stage)))))
-
-
-(define lhprobe-signedness-for-alist ((overridetype svar-overridetype-p)
-                                      (val svar/4vec-p)
-                                      ;; add config object?
-                                      )
-  ;; FIXME -- By default, it seems like it should mostly work to consider
-  ;; override-test variables signed and input/override-val variables unsigned.
-  ;; By convention, SVTV theorems usually set tests to -1 or 0 and assume other
-  ;; variables unsigned-byte-p of their widths.  Here we also detect whether an
-  ;; SVTV sets a signal to a non-zero-extended constant.  However, there's
-  ;; nothing forbidding an SVTV theorem from assuming some variables to be
-  ;; signed values.  In this case we might need to tweak the formula for
-  ;; determining signedness, and possibly add a configuration option for it.
-  (or (eq (svar-overridetype-fix overridetype) :test)
-      (and (svar/4vec-case val :4vec)
-           (or (< (4vec->upper val) 0)
-               (< (4vec->lower val) 0)))))
-
-(define svtv-spec-fsm-bindings-for-alist ((x svar/4vec-alist-p)
-                                             (stage natp)
-                                             (namemap svtv-name-lhs-map-p)
-                                             (overridetype svar-overridetype-p)
-                                             (bindings-acc lhprobe-map-p))
-  :returns (bindings lhprobe-map-p)
-  (b* (((when (atom x)) (lhprobe-map-fix bindings-acc))
-       ((unless (mbt (and (consp (car x)) (svar-p (caar x)))))
-        (svtv-spec-fsm-bindings-for-alist (cdr x) stage namemap overridetype bindings-acc))
-       ((cons var val) (car x))
-       (look (hons-get var (svtv-name-lhs-map-fix namemap)))
-       ((unless look)
-        (svtv-spec-fsm-bindings-for-alist (cdr x) stage namemap overridetype bindings-acc))
-       (lhs (cdr look))
-       (lhprobe (make-lhprobe :lhs (lhs-change-override lhs overridetype) :stage stage
-                              :signedp (lhprobe-signedness-for-alist overridetype val)))
-       (bindings-acc (svtv-spec-fsm-bindings-for-lhprobe lhprobe val bindings-acc)))
-    (svtv-spec-fsm-bindings-for-alist (cdr x) stage namemap overridetype bindings-acc))
-  ///
-  (local (in-theory (enable svar/4vec-alist-fix)))
-
-  (defret lhprobe-map-max-stage-of-<fn>
-    (implies (and (<= (nfix stage) bound)
-                  (<= (lhprobe-map-max-stage bindings-acc) bound))
-             (<= (lhprobe-map-max-stage bindings) bound))))
-
-(define svtv-spec-fsm-bindings-for-alists ((x svar/4vec-alistlist-p)
-                                           (stage natp)
-                                           (namemap svtv-name-lhs-map-p)
-                                           (overridetype svar-overridetype-p)
-                                           (bindings-acc lhprobe-map-p))
-  :returns (bindings lhprobe-map-p)
-  (if (atom x)
-      (lhprobe-map-fix bindings-acc)
-    (svtv-spec-fsm-bindings-for-alists
-     (cdr x) (1+ (lnfix stage)) namemap overridetype
-     (svtv-spec-fsm-bindings-for-alist (car x) stage namemap overridetype bindings-acc)))
-  ///
-  ;; (defret lhprobe-map-max-stage-of-<fn>
-  ;;   (<= (lhprobe-map-max-stage bindings) (max (+ (len x) (nfix stage))
-  ;;                                             (lhprobe-map-max-stage bindings-acc)))
-  ;;   :hints (("Goal" :induct t)
-  ;;           (and stable-under-simplificationp
-  ;;                '(:use ((:instance lhprobe-map-max-stage-of-svtv-spec-fsm-bindings-for-alist
-  ;;                         (x (car x))))
-  ;;                  :in-theory (disable lhprobe-map-max-stage-of-svtv-spec-fsm-bindings-for-alist))))
-  ;;   :rule-classes :linear)
-
-  (defret lhprobe-map-max-stage-of-<fn>
-    (implies (and (<= (+ -1 (len x) (nfix stage)) bound)
-                  (<= (lhprobe-map-max-stage bindings-acc) bound))
-             (<= (lhprobe-map-max-stage bindings) bound))))
-
-
-
-(define svtv-spec-fsm-bindings ((x svtv-spec-p))
-  :returns (bindings lhprobe-map-p)
-  :guard (svtv-spec-fsm-syntax-check x)
-  :guard-hints (("goal" :in-theory (enable svtv-spec-fsm-syntax-check)))
-  (b* (((svtv-spec x))
-       (len (len (svtv-probealist-outvars (svtv-spec->probes x))))
-       ((acl2::with-fast x.namemap))
-       (bindings (svtv-spec-fsm-bindings-for-alists (take len x.in-alists) 0 x.namemap nil nil))
-       (bindings (svtv-spec-fsm-bindings-for-alists (take len x.override-val-alists) 0 x.namemap :val bindings)))
-    (svtv-spec-fsm-bindings-for-alists (take len x.override-test-alists) 0 x.namemap :test bindings))
-  ///
-  (defret lhprobe-map-max-stage-of-<fn>
-    (<= (lhprobe-map-max-stage bindings) (1- (len (svtv-probealist-outvars (svtv-spec->probes x)))))
-    :rule-classes ((:linear :trigger-terms ((lhprobe-map-max-stage (svtv-spec-fsm-bindings x)))))))
-       
-
-
-
-
-
     
 
 
@@ -1486,39 +561,9 @@ to signed values.</p>"
 
 
 
-(define svtv-spec-fsm-constraints-for-lhprobe ((lhprobe lhprobe-p)
-                                               (binding svar/4vec-p)
-                                               (bindings lhprobe-map-p))
-  ;; Lhprobe is the LHS corresponding to some namemap name, which is mapped to binding in one of the input alists of the SVTV.
-
-  ;; Add constraints based on equating lhprobe and binding under the assumption
-  ;; that svtv variables are mapped to lhprobes as in bindings.
-
-  
-  
-  :returns (constraints lhprobe-constraintlist-p)
-  (svar/4vec-case binding
-    :4vec
-    ;; constant binding, add constraint
-    (list (make-lhprobe-constraint
-               :lhprobe lhprobe
-               :val (4vec-fix binding)))
-    :svar
-    ;; svtv variable, must have a binding
-    (b* ((binding-look (hons-get (svar-fix binding) (lhprobe-map-fix bindings)))
-         ((unless binding-look)
-          ;; add a constraint equating this hlprobe to x, I guess
-          (list (make-lhprobe-constraint
-                 :lhprobe lhprobe :val (4vec-x))))
-         (binding-lhprobe (cdr binding-look))
-         ((when (equal binding-lhprobe (lhprobe-fix lhprobe)))
-          ;; same, no constraint necessary
-          nil))
-      (list (make-lhprobe-constraint
-             :lhprobe lhprobe
-             :val binding-lhprobe))))
-  ///
-
+(defsection svtv-spec-fsm-constraints-for-lhprobe
+  (local (in-theory (enable svtv-spec-fsm-constraints-for-lhprobe)))
+  (local (std::set-define-current-function svtv-spec-fsm-constraints-for-lhprobe))
   (defret constraints-eval-of-<fn>
     (equal (lhprobe-constraintlist-eval constraints envs)
            (equal (lhprobe-eval lhprobe envs)
@@ -1567,41 +612,7 @@ to signed values.</p>"
 
 
 
-(defsection svex-envs-ovtestsimilar
-  ;; (def-universal-equiv svex-envs-ovtestsimilar
-  ;;   :qvars (k)
-  ;;   :equiv-terms ((4vec-1mask-equiv (svex-env-lookup k x))))
 
-  (defun-sk svex-envs-ovtestsimilar (x y)
-    (forall k
-            (implies (svar-override-p k :test)
-                     (4vec-1mask-equiv (svex-env-lookup k x)
-                                       (svex-env-lookup k y))))
-    :rewrite :direct)
-
-  (in-theory (disable svex-envs-ovtestsimilar
-                      svex-envs-ovtestsimilar-necc))
-
-  (defequiv svex-envs-ovtestsimilar
-    :hints ((and stable-under-simplificationp
-                 `(:expand (,(car (last clause)))
-                   :in-theory (enable svex-envs-ovtestsimilar-necc)))))
-
-  (defrefinement  svex-envs-similar svex-envs-ovtestsimilar
-    :hints(("Goal" :in-theory (enable svex-envs-ovtestsimilar)))))
-
-
-(define svex-envlists-ovtestsimilar ((x svex-envlist-p) (y svex-envlist-p))
-  (if (Atom x)
-      (atom y)
-    (and (consp y)
-         (ec-call (svex-envs-ovtestsimilar (car x) (car y)))
-         (svex-envlists-ovtestsimilar (cdr x) (cdr y))))
-  ///
-  (defequiv svex-envlists-ovtestsimilar)
-
-  (defrefinement svex-envlists-similar svex-envlists-ovtestsimilar
-    :hints(("Goal" :in-theory (enable svex-envlists-similar-rec)))))
 
 (defsection svex-envs-ovtestsubsetp
   (defun-sk svex-envs-ovtestsubsetp (x y)
@@ -1877,29 +888,9 @@ to signed values.</p>"
          (atom x))
   :hints(("Goal" :in-theory (enable lhs-width))))
 
-(define svtv-spec-fsm-constraints-for-alist ((x svar/4vec-alist-p)
-                                             (stage natp)
-                                             (namemap svtv-name-lhs-map-p)
-                                             (overridetype svar-overridetype-p)
-                                             (bindings lhprobe-map-p))
-  :returns (constraints lhprobe-constraintlist-p)
-
-  (b* (((when (atom x)) nil)
-       ((unless (mbt (and (consp (car x)) (svar-p (caar x)))))
-        (svtv-spec-fsm-constraints-for-alist (cdr x) stage namemap overridetype bindings))
-       ((cons var val) (car x))
-       (look (hons-get var (svtv-name-lhs-map-fix namemap)))
-       ((unless look)
-        (svtv-spec-fsm-constraints-for-alist (cdr x) stage namemap overridetype bindings))
-       (lhs (cdr look))
-       ;; FIXME -- See the comment about signedness in svtv-spec-fsm-bindings-for-alist.
-       ;; 
-       (lhprobe (make-lhprobe :lhs (lhs-change-override lhs overridetype) :stage stage
-                              :signedp (lhprobe-signedness-for-alist overridetype val))))
-    (append       
-     (svtv-spec-fsm-constraints-for-lhprobe lhprobe val bindings)
-     (svtv-spec-fsm-constraints-for-alist (cdr x) stage namemap overridetype bindings)))
-  ///
+(defsection svtv-spec-fsm-constraints-for-alist
+  (local (in-theory (enable svtv-spec-fsm-constraints-for-alist)))
+  (local (std::set-define-current-function svtv-spec-fsm-constraints-for-alist))
   (local (include-book "std/alists/fast-alist-clean" :dir :system))
   (local (include-book "std/lists/sets" :dir :system))
   (local (include-book "std/alists/fal-extract" :dir :system))
@@ -2495,51 +1486,10 @@ to signed values.</p>"
   (local (in-theory (enable svar/4vec-alist-fix))))
 
 
-(define svtv-fsm-namemap-envlist ((envs svex-envlist-p)
-                                  (map svtv-name-lhs-map-p)
-                                  (overridetype svar-overridetype-p))
-  :returns (stage-envs svex-envlist-p)
-  (if (atom envs)
-      nil
-    (cons (svtv-fsm-namemap-env (car envs) map overridetype)
-          (svtv-fsm-namemap-envlist (cdr envs) map overridetype))))
-
-(define svtv-fsm-namemap-alistlist ((alists svex-alistlist-p)
-                                    (map svtv-name-lhs-map-p)
-                                    (overridetype svar-overridetype-p))
-  :returns (stage-alists svex-alistlist-p)
-  (if (atom alists)
-      nil
-    (cons (svtv-fsm-namemap-alist-subst (car alists) map overridetype)
-          (svtv-fsm-namemap-alistlist (cdr alists) map overridetype))))
-
-(define svex-envlist-keys-list ((x svex-envlist-p))
-  :returns (vars svarlist-list-p)
-  (if (atom x)
-      nil
-    (cons  (alist-keys (svex-env-fix (car x)))
-           (svex-envlist-keys-list (cdr x))))
-  ///
-  (defthm svex-envlist-keys-list-of-svex-alistlist-eval
-    (equal (svex-envlist-keys-list (svex-alistlist-eval x env))
-           (svex-alist-keys-list x))
-    :hints(("Goal" :in-theory (enable svex-alist-keys-list
-                                      svex-alistlist-eval)))))
-
-
-(define svtv-spec-fsm-constraints-for-alists ((x svar/4vec-alistlist-p)
-                                              (stage natp)
-                                              (namemap svtv-name-lhs-map-p)
-                                              (overridetype svar-overridetype-p)
-                                              (bindings lhprobe-map-p))
-  :returns (constraints lhprobe-constraintlist-p)
-  (if (atom x)
-      nil
-    (append (svtv-spec-fsm-constraints-for-alist (car x) stage namemap overridetype bindings)
-            (svtv-spec-fsm-constraints-for-alists (cdr x) (1+ (lnfix stage)) namemap overridetype bindings)))
-  ///
-
-
+(defsection svtv-spec-fsm-constraints-for-alists
+  (local (in-theory (enable svtv-spec-fsm-constraints-for-alists)))
+  (local (std::set-define-current-function svtv-spec-fsm-constraints-for-alists))
+  
   (local (include-book "std/lists/nthcdr" :dir :system))
 
   (local (defun ind (in-alists val-alists test-alists stage)
@@ -2673,31 +1623,11 @@ to signed values.</p>"
                                          acl2::take-when-atom))))))
 
 
-(local (include-book "std/osets/element-list" :dir :system))
-(local (fty::deflist svarlist :elt-type svar :elementp-of-nil nil))
-
-(define svtv-spec-non-test-vars ((x svtv-spec-p))
-  :returns (vars svarlist-p)
-  (b* (((svtv-spec x))
-       (len (len (svtv-probealist-outvars x.probes)))
-       (ins (take len x.in-alists))
-       (vals (take len x.override-val-alists)))
-    (union (svex-alistlist-vars ins)
-           (svex-alistlist-vars vals))))
 
 
-(define svtv-spec-fsm-constraints ((x svtv-spec-p))
-  :returns (constraints lhprobe-constraintlist-p)
-  :guard (svtv-spec-fsm-syntax-check x)
-  :guard-hints (("goal" :in-theory (enable svtv-spec-fsm-syntax-check)))
-  (b* (((svtv-spec x))
-       (bindings (svtv-spec-fsm-bindings x))
-       (len (len (svtv-probealist-outvars (svtv-spec->probes x))))
-       ((acl2::with-fast x.namemap bindings)))
-    (append (svtv-spec-fsm-constraints-for-alists (take len x.in-alists) 0 x.namemap nil bindings)
-            (svtv-spec-fsm-constraints-for-alists (take len x.override-val-alists) 0 x.namemap :val bindings)))
-  ///
-
+(defsection svtv-spec-fsm-constraints
+  (local (in-theory (enable svtv-spec-fsm-constraints)))
+  (local (std::set-define-current-function svtv-spec-fsm-constraints))
   ;; Suppose we have an SVTV with an override-test set to -1 and the
   ;; corresponding override-val set to 0, and we want to show that FSM envs
   ;; without any overrride tests set comply with this.  The evaluation of the
@@ -3326,19 +2256,6 @@ to signed values.</p>"
 
 
 
-(define svtv-spec->override-test-alists* ((x svtv-spec-p))
-  (b* (((svtv-spec x)))
-    (take (len (svtv-probealist-outvars x.probes)) x.override-test-alists)))
-
-(define svtv-spec->override-val-alists* ((x svtv-spec-p))
-  (b* (((svtv-spec x)))
-    (take (len (svtv-probealist-outvars x.probes)) x.override-val-alists)))
-
-(define svtv-spec->in-alists* ((x svtv-spec-p))
-  (b* (((svtv-spec x)))
-    (take (len (svtv-probealist-outvars x.probes)) x.in-alists)))
-
-(define force-execute (x) x)
 
 (cmr::def-force-execute force-execute-force-execute force-execute)
 (in-theory (enable force-execute-force-execute))
@@ -4528,13 +3445,10 @@ to signed values.</p>"
 
 
 
-(define svtv-probe-to-lhprobe ((x svtv-probe-p)
-                               (namemap svtv-name-lhs-map-p))
-  :returns (lhprobe lhprobe-p)
-  (b* (((svtv-probe x)))
-    ;; This is used on the output side, and SVTV outputs are always unsigned (the LHSes are evaluated with lhs-eval-zero).
-    (make-lhprobe :stage x.time :lhs (cdr (hons-get x.signal (svtv-name-lhs-map-fix namemap)))))
-  ///
+(defsection svtv-probe-to-lhprobe
+  (local (in-theory (enable svtv-probe-to-lhprobe)))
+  (local (std::set-define-current-function svtv-probe-to-lhprobe))
+  
   (defret lhprobe-eval-of-<fn>
     (b* (((svtv-probe x)))
       (implies (hons-assoc-equal x.signal (svtv-name-lhs-map-fix namemap))
@@ -4562,16 +3476,9 @@ to signed values.</p>"
                                  svtv-probealist-vars)))))
 
 
-(define svtv-probealist-to-lhprobe-map ((x svtv-probealist-p)
-                                        (namemap svtv-name-lhs-map-p))
-  :returns (map lhprobe-map-p)
-  (if (atom x)
-      nil
-    (if (mbt (consp (car x)))
-        (cons (cons (svar-fix (caar x)) (svtv-probe-to-lhprobe (cdar x) namemap))
-              (svtv-probealist-to-lhprobe-map (cdr x) namemap))
-      (svtv-probealist-to-lhprobe-map (cdr x) namemap)))
-  ///
+(defsection svtv-probealist-to-lhprobe-map
+  (local (in-theory (enable svtv-probealist-to-lhprobe-map)))
+  (local (std::set-define-current-function svtv-probealist-to-lhprobe-map))
 
   (defret lhprobe-map-eval-of-<fn>
     (implies (and (subsetp-equal (svtv-probealist-vars x) (alist-keys (svtv-name-lhs-map-fix namemap)))
